Veir/Rewriter/WellFormed/Builder/Operation.lean
@@ -69,6 +69,5 @@ theorem Rewriter.createOp_WellFormed
   rename_i ctx₂ hctx₂
   have : ctx₂.WellFormed :=
     by grind [Rewriter.initOpRegions_WellFormed, IRContext.wellFormed_Rewriter_initOpResults]
-  sorry
-  -- grind [insertOp?_WellFormed, Rewriter.initOpOperands_WellFormed,
-  --   Rewriter.initBlockOperands_WellFormed]
+  grind [insertOp?_WellFormed, Rewriter.initOpOperands_WellFormed,
+    Rewriter.initBlockOperands_WellFormed]
